@prefix : <https://raw.githubusercontent.com/Salvadana/whata_ontology/main/ontology_development/whata_ontology.owl#> .
@prefix owl: <http://www.w3.org/2002/07/owl#> .
@prefix rdf: <http://www.w3.org/1999/02/22-rdf-syntax-ns#> .
@prefix xml: <http://www.w3.org/XML/1998/namespace> .
@prefix xsd: <http://www.w3.org/2001/XMLSchema#> .
@prefix rdfs: <http://www.w3.org/2000/01/rdf-schema#> .
@base <https://raw.githubusercontent.com/Salvadana/whata_ontology/main/ontology_development/whata_ontology.owl#> .

<https://raw.githubusercontent.com/Salvadana/whata_ontology/main/ontology_development/whata_ontology.owl> rdf:type owl:Ontology ;
                                                                                                           owl:imports <http://www.ontologydesignpatterns.org/ont/persp/perspectivisation.owl> .

#################################################################
#    Annotation properties
#################################################################

###  http://www.w3.org/2000/01/rdf-schema#subClassOf
rdfs:subClassOf rdf:type owl:AnnotationProperty .


#################################################################
#    Object Properties
#################################################################

###  https://raw.githubusercontent.com/Salvadana/whata_ontology/main/ontology_development/whata_ontology.owl#hasParticipant
:hasParticipant rdf:type owl:ObjectProperty ;
                owl:inverseOf :isParticipantIn ;
                rdfs:domain :BlameSituation ;
                rdfs:range :Ought ,
                           :ResponsibilityOwner .


###  https://raw.githubusercontent.com/Salvadana/whata_ontology/main/ontology_development/whata_ontology.owl#isParticipantIn
:isParticipantIn rdf:type owl:ObjectProperty ;
                 rdfs:domain :Ought ,
                             :ResponsibilityOwner ;
                 rdfs:range :BlameSituation .


###  https://raw.githubusercontent.com/Salvadana/whata_ontology/main/ontology_development/whata_ontology.owl#relatedToLens
:relatedToLens rdf:type owl:ObjectProperty ;
               rdfs:domain :FocusShiftingLens ;
               rdfs:range :FocusShiftingLens .


###  https://raw.githubusercontent.com/Salvadana/whata_ontology/main/ontology_development/whata_ontology.owl#shiftsFocusFrom
:shiftsFocusFrom rdf:type owl:ObjectProperty ;
                 rdfs:domain :FocusShiftingLens ;
                 rdfs:range <http://www.ontologydesignpatterns.org/ont/persp/perspectivisation.owl#Eventuality> .


#################################################################
#    Data properties
#################################################################

###  https://raw.githubusercontent.com/Salvadana/whata_ontology/main/ontology_development/whata_ontology.owl#relatedIdentifyingPattern
:relatedIdentifyingPattern rdf:type owl:DatatypeProperty ;
                           rdfs:domain :WhataboutistPerspectivisation ;
                           rdfs:range xsd:string .


#################################################################
#    Classes
#################################################################

###  http://www.ontologydesignpatterns.org/ont/persp/perspectivisation.owl#Attitude
<http://www.ontologydesignpatterns.org/ont/persp/perspectivisation.owl#Attitude> rdfs:subClassOf <http://www.ontologydesignpatterns.org/ont/persp/perspectivisation.owl#PerspectivisationTheorySituation> .


###  http://www.ontologydesignpatterns.org/ont/persp/perspectivisation.owl#Lens
<http://www.ontologydesignpatterns.org/ont/persp/perspectivisation.owl#Lens> rdfs:subClassOf <http://www.ontologydesignpatterns.org/ont/persp/perspectivisation.owl#PerspectivisationTheorySituation> .


###  https://raw.githubusercontent.com/Salvadana/whata_ontology/main/ontology_development/whata_ontology.owl#Blamable
:Blamable rdf:type owl:Class ;
          rdfs:subClassOf <http://www.ontologydesignpatterns.org/ont/persp/perspectivisation.owl#Blendable> ,
                          <http://www.ontologydesignpatterns.org/ont/persp/perspectivisation.owl#Eventuality> ,
                          :BlameSituation .


###  https://raw.githubusercontent.com/Salvadana/whata_ontology/main/ontology_development/whata_ontology.owl#BlameSituation
:BlameSituation rdf:type owl:Class ;
                rdfs:subClassOf <http://www.ontologydesignpatterns.org/ont/persp/perspectivisation.owl#Blending> .


###  https://raw.githubusercontent.com/Salvadana/whata_ontology/main/ontology_development/whata_ontology.owl#BlendedBlameBackground
:BlendedBlameBackground rdf:type owl:Class ;
                        rdfs:subClassOf <http://www.ontologydesignpatterns.org/ont/persp/perspectivisation.owl#Background> ,
                                        <http://www.ontologydesignpatterns.org/ont/persp/perspectivisation.owl#Blended> ,
                                        :BlameSituation .


###  https://raw.githubusercontent.com/Salvadana/whata_ontology/main/ontology_development/whata_ontology.owl#ConfirmationBiasLens
:ConfirmationBiasLens rdf:type owl:Class ;
                      rdfs:subClassOf :FocusShiftingLens ;
                      rdfs:comment "The Confirmation Bias Lens is a focus shifting lens." .


###  https://raw.githubusercontent.com/Salvadana/whata_ontology/main/ontology_development/whata_ontology.owl#CounterBlamable
:CounterBlamable rdf:type owl:Class ;
                 rdfs:subClassOf <http://www.ontologydesignpatterns.org/ont/persp/perspectivisation.owl#Blendable> ,
                                 <http://www.ontologydesignpatterns.org/ont/persp/perspectivisation.owl#Cut> ,
                                 :BlameSituation .


###  https://raw.githubusercontent.com/Salvadana/whata_ontology/main/ontology_development/whata_ontology.owl#FocusShiftingLens
:FocusShiftingLens rdf:type owl:Class ;
                   rdfs:subClassOf <http://www.ontologydesignpatterns.org/ont/persp/perspectivisation.owl#Lens> ;
                   rdfs:comment "The focus shifting lens is the lens responsible for a focus shift within a perspectivisation." .


###  https://raw.githubusercontent.com/Salvadana/whata_ontology/main/ontology_development/whata_ontology.owl#Ought
:Ought rdf:type owl:Class .


###  https://raw.githubusercontent.com/Salvadana/whata_ontology/main/ontology_development/whata_ontology.owl#RelevanceFallacyLens
:RelevanceFallacyLens rdf:type owl:Class ;
                      rdfs:subClassOf :FocusShiftingLens ;
                      rdfs:comment "The RelevanceFallacyLens is a Focus Shifting Lens." .


###  https://raw.githubusercontent.com/Salvadana/whata_ontology/main/ontology_development/whata_ontology.owl#ResponsibilityOwner
:ResponsibilityOwner rdf:type owl:Class ;
                     rdfs:subClassOf <http://www.ontologydesignpatterns.org/cp/owl/agentrole.owl#Agent> ;
                     rdfs:comment "The Responsibility Owner is the entity owning a certain responsibility towards a Ought within a Blame situation." .


###  https://raw.githubusercontent.com/Salvadana/whata_ontology/main/ontology_development/whata_ontology.owl#WhataboutistLens
:WhataboutistLens rdf:type owl:Class ;
                  rdfs:subClassOf :FocusShiftingLens .


###  https://raw.githubusercontent.com/Salvadana/whata_ontology/main/ontology_development/whata_ontology.owl#WhataboutistPerspectivisation
:WhataboutistPerspectivisation rdf:type owl:Class ;
                               rdfs:subClassOf <http://www.ontologydesignpatterns.org/ont/persp/perspectivisation.owl#Perspectivisation> .


#################################################################
#    Individuals
#################################################################

###  https://raw.githubusercontent.com/Salvadana/whata_ontology/main/ontology_development/whata_ontology.owl#Blamable
:Blamable rdf:type owl:NamedIndividual ,
                   :Blamable .


###  https://raw.githubusercontent.com/Salvadana/whata_ontology/main/ontology_development/whata_ontology.owl#BlameSituation
:BlameSituation rdf:type owl:NamedIndividual .


###  https://raw.githubusercontent.com/Salvadana/whata_ontology/main/ontology_development/whata_ontology.owl#BlendedBlameBackground
:BlendedBlameBackground rdf:type owl:NamedIndividual ,
                                 :BlendedBlameBackground .


###  https://raw.githubusercontent.com/Salvadana/whata_ontology/main/ontology_development/whata_ontology.owl#ConfirmationBias
:ConfirmationBias rdf:type owl:NamedIndividual ,
                           :ConfirmationBiasLens ;
                  :relatedToLens :WhataboutistLens .


###  https://raw.githubusercontent.com/Salvadana/whata_ontology/main/ontology_development/whata_ontology.owl#CounterBlamable
:CounterBlamable rdf:type owl:NamedIndividual ,
                          :CounterBlamable ;
                 <http://www.ontologydesignpatterns.org/ont/persp/perspectivisation.owl#shotThrough> :WhataboutistLens .


###  https://raw.githubusercontent.com/Salvadana/whata_ontology/main/ontology_development/whata_ontology.owl#Ought
:Ought rdf:type owl:NamedIndividual ,
                :Ought ;
       :isParticipantIn :Blamable ,
                        :BlendedBlameBackground ,
                        :CounterBlamable .


###  https://raw.githubusercontent.com/Salvadana/whata_ontology/main/ontology_development/whata_ontology.owl#ResponsibilityOwner1
:ResponsibilityOwner1 rdf:type owl:NamedIndividual ,
                               :ResponsibilityOwner ;
                      :isParticipantIn :Blamable ,
                                       :BlendedBlameBackground .


###  https://raw.githubusercontent.com/Salvadana/whata_ontology/main/ontology_development/whata_ontology.owl#ResponsibilityOwner2
:ResponsibilityOwner2 rdf:type owl:NamedIndividual ,
                               :ResponsibilityOwner ;
                      :isParticipantIn :BlendedBlameBackground ,
                                       :CounterBlamable .


###  https://raw.githubusercontent.com/Salvadana/whata_ontology/main/ontology_development/whata_ontology.owl#TuQuoqueFallacy
:TuQuoqueFallacy rdf:type owl:NamedIndividual ,
                          :RelevanceFallacyLens ;
                 :relatedToLens :WhataboutistLens .


###  https://raw.githubusercontent.com/Salvadana/whata_ontology/main/ontology_development/whata_ontology.owl#WhataboutistLens
:WhataboutistLens rdf:type owl:NamedIndividual ,
                           :WhataboutistLens ;
                  :shiftsFocusFrom :Blamable .


###  https://raw.githubusercontent.com/Salvadana/whata_ontology/main/ontology_development/whata_ontology.owl#WhataboutistPerspectivisation
:WhataboutistPerspectivisation rdf:type owl:NamedIndividual ,
                                        :WhataboutistPerspectivisation ;
                               <http://www.ontologydesignpatterns.org/ont/persp/perspectivisation.owl#Background> :BlendedBlameBackground ;
                               <http://www.ontologydesignpatterns.org/ont/persp/perspectivisation.owl#Cut> :CounterBlamable ;
                               <http://www.ontologydesignpatterns.org/ont/persp/perspectivisation.owl#Eventuality> :Blamable ;
                               <http://www.ontologydesignpatterns.org/ont/persp/perspectivisation.owl#Lens> :WhataboutistLens ;
                               :relatedIdentifyingPattern "what about" .


#################################################################
#    Annotations
#################################################################

:Blamable rdfs:comment "The Blamable is the Eventuality the focus is shift from in a Whataboutist Perspectivisation. It is blendable with a CounterBlamable eventuality within a conceptual blending operation." .


:BlameSituation rdfs:comment "The Blame Situation represents the element blending the Blamable situation with the CounterBlamable situation." .


:BlendedBlameBackground rdfs:comment "The BlendedBlameBackground is the enlarged background used in a WhataboutistPerspectivisation. It is a blended space resulting from the conceptual blanding of the Blamable and the CounterBlamable situation." .


:CounterBlamable rdfs:comment "The CounterBlamable represents the Cut shot through the Whataboutist Lens. It is blendable with a Blamable eventuality within a conceptual blending operation." .


:Ought rdfs:comment "The Ought represents the shared norm, due or value that is addressed in the Blame Situation." .


:WhataboutistLens rdfs:comment "The Whataboutist Lens is the Focus Shifting Lens which is responsible for the focus shift within a Whataboutist Perspectivisation. It shifts the focus from a blamable eventuality and tailors the CounterBlamable Cut within the perspectivisation." .


:WhataboutistPerspectivisation rdfs:comment "The Whataboutist Perspectivisation is the perspectivisation characterised by a Whataboutis Lens that shifts the focus from a Blamable situation towards a CounterBlamable situation having as Background the blended space resulting from the blending of the Blamable and the CounterBlamable." .


###  Generated by the OWL API (version 5.1.18) https://github.com/owlcs/owlapi/
