Prefix(:=<https://raw.githubusercontent.com/Salvadana/whata_ontology/main/ontology_development/whata_ontology.owl#>)
Prefix(owl:=<http://www.w3.org/2002/07/owl#>)
Prefix(rdf:=<http://www.w3.org/1999/02/22-rdf-syntax-ns#>)
Prefix(xml:=<http://www.w3.org/XML/1998/namespace>)
Prefix(xsd:=<http://www.w3.org/2001/XMLSchema#>)
Prefix(rdfs:=<http://www.w3.org/2000/01/rdf-schema#>)


Ontology(<https://raw.githubusercontent.com/Salvadana/whata_ontology/main/ontology_development/whata_ontology.owl>
Import(<http://www.ontologydesignpatterns.org/ont/persp/perspectivisation.owl>)

Declaration(Class(:Blamable))
Declaration(Class(:BlameSituation))
Declaration(Class(:BlendedBlameBackground))
Declaration(Class(:ConfirmationBiasLens))
Declaration(Class(:CounterBlamable))
Declaration(Class(:FocusShiftingLens))
Declaration(Class(:Ought))
Declaration(Class(:RelevanceFallacyLens))
Declaration(Class(:ResponsibilityOwner))
Declaration(Class(:WhataboutistLens))
Declaration(Class(:WhataboutistPerspectivisation))
Declaration(ObjectProperty(:hasParticipant))
Declaration(ObjectProperty(:isParticipantIn))
Declaration(ObjectProperty(:relatedToLens))
Declaration(ObjectProperty(:shiftsFocusFrom))
Declaration(DataProperty(:relatedIdentifyingPattern))
Declaration(NamedIndividual(:Blamable))
Declaration(NamedIndividual(:BlameSituation))
Declaration(NamedIndividual(:BlendedBlameBackground))
Declaration(NamedIndividual(:ConfirmationBias))
Declaration(NamedIndividual(:CounterBlamable))
Declaration(NamedIndividual(:Ought))
Declaration(NamedIndividual(:ResponsibilityOwner1))
Declaration(NamedIndividual(:ResponsibilityOwner2))
Declaration(NamedIndividual(:TuQuoqueFallacy))
Declaration(NamedIndividual(:WhataboutistLens))
Declaration(NamedIndividual(:WhataboutistPerspectivisation))
Declaration(AnnotationProperty(rdfs:subClassOf))

############################
#   Object Properties
############################

# Object Property: :hasParticipant (:hasParticipant)

InverseObjectProperties(:hasParticipant :isParticipantIn)
ObjectPropertyDomain(:hasParticipant :BlameSituation)
ObjectPropertyRange(:hasParticipant :Ought)
ObjectPropertyRange(:hasParticipant :ResponsibilityOwner)

# Object Property: :isParticipantIn (:isParticipantIn)

ObjectPropertyDomain(:isParticipantIn :Ought)
ObjectPropertyDomain(:isParticipantIn :ResponsibilityOwner)
ObjectPropertyRange(:isParticipantIn :BlameSituation)

# Object Property: :relatedToLens (:relatedToLens)

ObjectPropertyDomain(:relatedToLens :FocusShiftingLens)
ObjectPropertyRange(:relatedToLens :FocusShiftingLens)

# Object Property: :shiftsFocusFrom (:shiftsFocusFrom)

ObjectPropertyDomain(:shiftsFocusFrom :FocusShiftingLens)
ObjectPropertyRange(:shiftsFocusFrom <http://www.ontologydesignpatterns.org/ont/persp/perspectivisation.owl#Eventuality>)


############################
#   Data Properties
############################

# Data Property: :relatedIdentifyingPattern (:relatedIdentifyingPattern)

DataPropertyDomain(:relatedIdentifyingPattern :WhataboutistPerspectivisation)
DataPropertyRange(:relatedIdentifyingPattern xsd:string)



############################
#   Classes
############################

# Class: <http://www.ontologydesignpatterns.org/ont/persp/perspectivisation.owl#Attitude> (<http://www.ontologydesignpatterns.org/ont/persp/perspectivisation.owl#Attitude>)

SubClassOf(<http://www.ontologydesignpatterns.org/ont/persp/perspectivisation.owl#Attitude> <http://www.ontologydesignpatterns.org/ont/persp/perspectivisation.owl#PerspectivisationTheorySituation>)

# Class: <http://www.ontologydesignpatterns.org/ont/persp/perspectivisation.owl#Lens> (<http://www.ontologydesignpatterns.org/ont/persp/perspectivisation.owl#Lens>)

SubClassOf(<http://www.ontologydesignpatterns.org/ont/persp/perspectivisation.owl#Lens> <http://www.ontologydesignpatterns.org/ont/persp/perspectivisation.owl#PerspectivisationTheorySituation>)

# Class: :Blamable (:Blamable)

AnnotationAssertion(rdfs:comment :Blamable "The Blamable is the Eventuality the focus is shift from in a Whataboutist Perspectivisation. It is blendable with a CounterBlamable eventuality within a conceptual blending operation.")
SubClassOf(:Blamable <http://www.ontologydesignpatterns.org/ont/persp/perspectivisation.owl#Blendable>)
SubClassOf(:Blamable <http://www.ontologydesignpatterns.org/ont/persp/perspectivisation.owl#Eventuality>)
SubClassOf(:Blamable :BlameSituation)

# Class: :BlameSituation (:BlameSituation)

AnnotationAssertion(rdfs:comment :BlameSituation "The Blame Situation represents the element blending the Blamable situation with the CounterBlamable situation.")
SubClassOf(:BlameSituation <http://www.ontologydesignpatterns.org/ont/persp/perspectivisation.owl#Blending>)

# Class: :BlendedBlameBackground (:BlendedBlameBackground)

AnnotationAssertion(rdfs:comment :BlendedBlameBackground "The BlendedBlameBackground is the enlarged background used in a WhataboutistPerspectivisation. It is a blended space resulting from the conceptual blanding of the Blamable and the CounterBlamable situation.")
SubClassOf(:BlendedBlameBackground <http://www.ontologydesignpatterns.org/ont/persp/perspectivisation.owl#Background>)
SubClassOf(:BlendedBlameBackground <http://www.ontologydesignpatterns.org/ont/persp/perspectivisation.owl#Blended>)
SubClassOf(:BlendedBlameBackground :BlameSituation)

# Class: :ConfirmationBiasLens (:ConfirmationBiasLens)

AnnotationAssertion(rdfs:comment :ConfirmationBiasLens "The Confirmation Bias Lens is a focus shifting lens.")
SubClassOf(:ConfirmationBiasLens :FocusShiftingLens)

# Class: :CounterBlamable (:CounterBlamable)

AnnotationAssertion(rdfs:comment :CounterBlamable "The CounterBlamable represents the Cut shot through the Whataboutist Lens. It is blendable with a Blamable eventuality within a conceptual blending operation.")
SubClassOf(:CounterBlamable <http://www.ontologydesignpatterns.org/ont/persp/perspectivisation.owl#Blendable>)
SubClassOf(:CounterBlamable <http://www.ontologydesignpatterns.org/ont/persp/perspectivisation.owl#Cut>)
SubClassOf(:CounterBlamable :BlameSituation)

# Class: :FocusShiftingLens (:FocusShiftingLens)

AnnotationAssertion(rdfs:comment :FocusShiftingLens "The focus shifting lens is the lens responsible for a focus shift within a perspectivisation.")
SubClassOf(:FocusShiftingLens <http://www.ontologydesignpatterns.org/ont/persp/perspectivisation.owl#Lens>)

# Class: :Ought (:Ought)

AnnotationAssertion(rdfs:comment :Ought "The Ought represents the shared norm, due or value that is addressed in the Blame Situation.")

# Class: :RelevanceFallacyLens (:RelevanceFallacyLens)

AnnotationAssertion(rdfs:comment :RelevanceFallacyLens "The RelevanceFallacyLens is a Focus Shifting Lens.")
SubClassOf(:RelevanceFallacyLens :FocusShiftingLens)

# Class: :ResponsibilityOwner (:ResponsibilityOwner)

AnnotationAssertion(rdfs:comment :ResponsibilityOwner "The Responsibility Owner is the entity owning a certain responsibility towards a Ought within a Blame situation.")
SubClassOf(:ResponsibilityOwner <http://www.ontologydesignpatterns.org/cp/owl/agentrole.owl#Agent>)

# Class: :WhataboutistLens (:WhataboutistLens)

AnnotationAssertion(rdfs:comment :WhataboutistLens "The Whataboutist Lens is the Focus Shifting Lens which is responsible for the focus shift within a Whataboutist Perspectivisation. It shifts the focus from a blamable eventuality and tailors the CounterBlamable Cut within the perspectivisation.")
SubClassOf(:WhataboutistLens :FocusShiftingLens)

# Class: :WhataboutistPerspectivisation (:WhataboutistPerspectivisation)

AnnotationAssertion(rdfs:comment :WhataboutistPerspectivisation "The Whataboutist Perspectivisation is the perspectivisation characterised by a Whataboutis Lens that shifts the focus from a Blamable situation towards a CounterBlamable situation having as Background the blended space resulting from the blending of the Blamable and the CounterBlamable.")
SubClassOf(:WhataboutistPerspectivisation <http://www.ontologydesignpatterns.org/ont/persp/perspectivisation.owl#Perspectivisation>)


############################
#   Named Individuals
############################

# Individual: :Blamable (:Blamable)

ClassAssertion(:Blamable :Blamable)

# Individual: :BlendedBlameBackground (:BlendedBlameBackground)

ClassAssertion(:BlendedBlameBackground :BlendedBlameBackground)

# Individual: :ConfirmationBias (:ConfirmationBias)

ClassAssertion(:ConfirmationBiasLens :ConfirmationBias)
ObjectPropertyAssertion(:relatedToLens :ConfirmationBias :WhataboutistLens)

# Individual: :CounterBlamable (:CounterBlamable)

ClassAssertion(:CounterBlamable :CounterBlamable)
ObjectPropertyAssertion(<http://www.ontologydesignpatterns.org/ont/persp/perspectivisation.owl#shotThrough> :CounterBlamable :WhataboutistLens)

# Individual: :Ought (:Ought)

ClassAssertion(:Ought :Ought)
ObjectPropertyAssertion(:isParticipantIn :Ought :Blamable)
ObjectPropertyAssertion(:isParticipantIn :Ought :BlendedBlameBackground)
ObjectPropertyAssertion(:isParticipantIn :Ought :CounterBlamable)

# Individual: :ResponsibilityOwner1 (:ResponsibilityOwner1)

ClassAssertion(:ResponsibilityOwner :ResponsibilityOwner1)
ObjectPropertyAssertion(:isParticipantIn :ResponsibilityOwner1 :Blamable)
ObjectPropertyAssertion(:isParticipantIn :ResponsibilityOwner1 :BlendedBlameBackground)

# Individual: :ResponsibilityOwner2 (:ResponsibilityOwner2)

ClassAssertion(:ResponsibilityOwner :ResponsibilityOwner2)
ObjectPropertyAssertion(:isParticipantIn :ResponsibilityOwner2 :BlendedBlameBackground)
ObjectPropertyAssertion(:isParticipantIn :ResponsibilityOwner2 :CounterBlamable)

# Individual: :TuQuoqueFallacy (:TuQuoqueFallacy)

ClassAssertion(:RelevanceFallacyLens :TuQuoqueFallacy)
ObjectPropertyAssertion(:relatedToLens :TuQuoqueFallacy :WhataboutistLens)

# Individual: :WhataboutistLens (:WhataboutistLens)

ClassAssertion(:WhataboutistLens :WhataboutistLens)
ObjectPropertyAssertion(:shiftsFocusFrom :WhataboutistLens :Blamable)

# Individual: :WhataboutistPerspectivisation (:WhataboutistPerspectivisation)

ClassAssertion(:WhataboutistPerspectivisation :WhataboutistPerspectivisation)
ObjectPropertyAssertion(<http://www.ontologydesignpatterns.org/ont/persp/perspectivisation.owl#Background> :WhataboutistPerspectivisation :BlendedBlameBackground)
ObjectPropertyAssertion(<http://www.ontologydesignpatterns.org/ont/persp/perspectivisation.owl#Cut> :WhataboutistPerspectivisation :CounterBlamable)
ObjectPropertyAssertion(<http://www.ontologydesignpatterns.org/ont/persp/perspectivisation.owl#Eventuality> :WhataboutistPerspectivisation :Blamable)
ObjectPropertyAssertion(<http://www.ontologydesignpatterns.org/ont/persp/perspectivisation.owl#Lens> :WhataboutistPerspectivisation :WhataboutistLens)
DataPropertyAssertion(:relatedIdentifyingPattern :WhataboutistPerspectivisation "what about")


)